Nvalues defined on literals (old syntax was modified), function that check if a fun have al the variables bounded was added, value tree and sensors state updated

expression.v
@@ -2,9 +2,8 @@ Set Warnings "-notation-overridden,-parsing,-deprecated-hint-without-locality".
 From Coq Require Import Strings.String.
 Require Import PeanoNat.
 Require Import nvalue.
-Require Import value_tree.
 Require Import Bool.
-
+Require Import List.
 
 Inductive ty : Type :=
   | Ty_Builtin : Type -> ty
@@ -12,17 +11,19 @@ Inductive ty : Type :=
 
 Inductive exp: Type :=
   | exp_var : string -> exp
-  | exp_abs : string -> string -> ty -> exp -> exp
   | exp_app : exp -> exp -> exp
   | exp_val : string -> exp -> exp -> exp
   | exp_if : exp -> exp -> exp -> exp
-  | exp_nvalue (A:Type) : nvalue A -> exp
-  | l_true : exp
-  | l_false : exp
-  | l_const : nat -> exp
-  | l_succ : exp -> exp
-  | l_pred : exp -> exp 
-  | l_mult : exp -> exp -> exp.
+  | exp_nvalue : nvalue literal-> exp
+  | exp_literal : literal -> exp
+with literal :=
+  | l_true : literal
+  | l_false : literal
+  | l_const : nat -> literal
+  | l_succ : exp -> literal
+  | l_pred : exp -> literal 
+  | l_mult : exp -> exp -> literal
+  | l_abs : string -> string -> ty -> exp -> literal.
 
 Declare Custom Entry acnotation.
 
@@ -34,7 +35,7 @@ Coercion exp_var : string >-> exp.
 
 (*lambda*)
 Notation "'fun' name [ x :  t ]  { y }" :=
-  (exp_abs name x t y) (in custom acnotation at level 90, 
+  (l_abs name x t y) (in custom acnotation at level 90, 
                      name at level 99,
                      x at level 99,
                      t custom acnotation at level 99,
@@ -70,7 +71,10 @@ Notation "'pred' x" := (l_pred x) (in custom acnotation at level 0,
                                      x custom acnotation at level 0).
 Notation "x * y" := (l_mult x y) (in custom acnotation at level 1,
                                       left associativity).
-Coercion l_const: nat >-> exp.
+
+Coercion exp_literal: literal >-> exp.
+Coercion l_const: nat >-> literal.
+
 
 (*if condition*)
 Notation "'if' x 'then' y 'else' z" :=
@@ -81,14 +85,13 @@ Notation "'if' x 'then' y 'else' z" :=
                     left associativity).
 
 (*nvalues*)
-Notation "[ > l ]" := (default _ l) (in custom acnotation at level 30).
-Notation "[ x >> y ] m" := ( device _ x y m)(in custom acnotation at level 30,
+Notation "[ > l ]" := (default literal l) (in custom acnotation at level 30).
+Notation "[ x >> y ] m" := ( device literal x y m)(in custom acnotation at level 30,
                                             x at level 99, 
                                             y at level 99, 
                                             m custom acnotation at level 30).
 
 Coercion exp_nvalue: nvalue >-> exp.
-Notation "'NvalueNat'" := (Ty_Builtin (nvalue nat)) (in custom acnotation at level 0).
 
 
 Inductive value : exp -> Prop :=
@@ -99,7 +102,8 @@ Inductive value : exp -> Prop :=
   | v_false :
       value <{false}>
   | v_nat: forall (n:nat), value <{n}>
-  | v_nvalue: forall (A:Type) (n:nvalue A), value <{n}>.
+  | v_nvalue: forall (n:nvalue literal), value <{n}>.
+Hint Constructors value : core.
 
 Reserved Notation "'/' x ':=' s '/' t" (in custom acnotation at level 20, x constr).
 Fixpoint subst (x : string) (s : exp) (t : exp) : exp :=
@@ -114,7 +118,7 @@ Fixpoint subst (x : string) (s : exp) (t : exp) : exp :=
       if (String.eqb x n) then t else <{val n = (/x:=s/ t1) ; (/x:=s/ t2)}>
   | <{if t1 then t2 else t3}> =>
         <{if (/x:=s/ t1) then (/x:=s/ t2) else (/x:=s/ t3)}>
-  | exp_nvalue x nv =>
+  | exp_nvalue nv =>
     <{nv}>
   | <{true}> =>
       <{true}>
@@ -130,88 +134,39 @@ Fixpoint subst (x : string) (s : exp) (t : exp) : exp :=
     <{(/x:=s/ t1) * (/x:=s/ t2)}>
   end
 where "'/' x ':=' s '/' t" := (subst x s t) (in custom acnotation).
-Hint Constructors value : core.
 
-Reserved Notation "t '-->' t'" (at level 40). 
-Inductive step : exp -> exp -> Prop :=
-  | ST_AppAbs : forall n x T2 t1 v2,
-         value v2 ->
-         <{(fun n [x:T2] {t1}) v2}> --> <{ /n:=(fun n [x:T2] {t1})/ /x:=v2/ t1 }>
-  | ST_App1 : forall t1 t1' t2,
-         t1 --> t1' ->
-         <{t1 t2}> --> <{t1' t2}>
-  | ST_App2 : forall v1 t2 t2',
-         value v1 ->
-         t2 --> t2' ->
-         <{v1 t2}> --> <{v1 t2'}>
-  | ST_IfTrue : forall t1 t2,
-      <{if true then t1 else t2}> --> t1
-  | ST_IfFalse : forall t1 t2,
-      <{if false then t1 else t2}> --> t2
-  | ST_If : forall t1 t1' t2 t3,
-      t1 --> t1' ->
-      <{if t1 then t2 else t3}> --> <{if t1' then t2 else t3}>
-  | ST_succ: forall (n:nat) (m:nat), m = S n -> <{succ n}> --> <{m}>
-  | ST_succ_step: forall t t',  t --> t' -> <{succ t}> --> <{succ t'}>
-  | ST_pred: forall (n:nat) (m:nat), m = Nat.pred n -> <{pred n}> --> <{m}>
-  | ST_pred_step: forall t t',  t --> t' -> <{pred t}> --> <{pred t'}>
-  | ST_prod: forall (n:nat) (m:nat) (r:nat), r = n * m -> <{n * m}> --> <{r}>
-  | ST_prod_left: forall (n:nat) (n':nat) (m:nat), n --> n' -> <{n * m}> --> <{n' * m}>
-  | ST_prod_right: forall (n:nat) (m:nat) (m':nat), m --> m' -> <{n * m}> --> <{n * m'}>
-  | ST_Let1: forall n t1 t1' t2, t1 --> t1' -> 
-            <{val n = t1 ; t2}> --> <{val n = t1' ; t2}>
-  | ST_LetValue: forall n v1 t2, value v1 -> <{val n = v1 ; t2}> --> <{ /n:=v1/t2}>
-where "t '-->' t'" := (step t t').
-
-(*multi-step*)
-Definition relation (X : Type) := X -> X -> Prop.
-Inductive multi {X : Type} (R : relation X) : relation X :=
-  | multi_refl : forall (x : X), multi R x x
-  | multi_single : forall (x y: X), R x y -> multi R x y
-  | multi_step : forall (x y z : X),
-                    R x y ->
-                    multi R y z ->
-                    multi R x z.
-Notation multistep := (multi step).
-Notation "t1 '-->*' t2" := (multistep t1 t2) (at level 40).
+Fixpoint bounded (e:exp) (l_bounded:list string): Prop :=
+match e with 
+  | exp_var y =>
+    In y l_bounded
+  | <{fun n [y:T] {t1}}> =>
+    bounded t1 (cons y l_bounded)
+  | <{t1 t2}> =>
+    (bounded t1 l_bounded) /\ (bounded t1 l_bounded)
+  | <{val n = t1 ; t2}> =>
+    (bounded t1 l_bounded(*(cons n l_bounded)*)) /\ (bounded t2 (cons n l_bounded))
+  | <{if t1 then t2 else t3}> =>
+    (bounded t1 l_bounded) /\ (bounded t2 l_bounded)
+    /\ (bounded t3 l_bounded)
+  | exp_nvalue nv =>
+    True
+  | <{true}> =>
+    False
+  | <{false}> =>
+    True
+  | l_const n =>
+    False
+  | l_succ t1 =>
+    (bounded t1 l_bounded)
+  | l_pred t1 =>
+    (bounded t1 l_bounded)
+  | l_mult t1 t2 =>
+    (bounded t1 l_bounded) /\ (bounded t2 l_bounded)
+end. 
 
 
-Reserved Notation "t '==>' t'" (at level 40).
-Inductive bigstep : exp -> exp -> Prop :=
-  | ST_Val : forall n t1 t2 w1 w2,
-    <{t1}> ==> <{w1}> ->
-    <{/n := w1/ t2 }> ==> <{w2}> ->
-    <{val n = t1 ; t2}> ==> <{w2}>
-  | ST_App : forall v t1 t2' t2 w,
-    value v ->
-    <{t1}> ==> v ->
-    <{t2}> ==> <{t2'}> ->
-    <{v t2'}> ==> <{w}> ->
-    <{t1 t2}> ==> <{w}>
-  | ST_Fun : forall n x T2 t1 v w,
-    value v ->
-    <{ /n:=(fun n [x:T2] {t1})/ /x:=v/ t1 }> ==> <{w}> ->
-    <{(fun n [x:T2] {t1}) v}> ==> <{w}>
-  | ST_Succ: forall (n:nat) w e, 
-    w = S n ->
-    <{e}> ==> <{n}> ->
-    <{succ e}> ==> <{w}>
-  | ST_Pred: forall (n:nat) w e, 
-    w = Nat.pred n ->
-    <{e}> ==> <{n}> ->
-    <{pred e}> ==> <{w}>
-  | ST_Prod: forall n (n':nat) m (m':nat) w, 
-    w = n' * m' ->
-    <{n}> ==> <{n'}> ->
-    <{m}> ==> <{m'}> ->
-    <{n * m}> ==> <{w}>
-  | ST_If_T: forall t1 t2 t3,
-    <{t1}> ==> <{true}> ->
-    <{if t1 then t2 else t3}> ==> <{t2}>
-  | ST_If_F: forall t1 t2 t3,
-    <{t1}> ==> <{false}> ->
-    <{if t1 then t2 else t3}> ==> <{t3}>
-  | ST_Refl: forall t1, <{t1}> ==> <{t1}>
-where "t '==>' t'" := (bigstep t t').
+
+
+
 
 
