big_step_semantics.v
@@ -1,0 +1,50 @@
+Require Import expression.
+Require Import sensor_state.
+Require Import value_tree.
+Require Import nvalue.
+Require Import Bool.
+Require Import String.
+Require Import List.
+
+Variable Delta : nat.
+Variable Sigma : sensor_state.
+Variable VtEnvironment : value_tree_env.
+
+
+Reserved Notation "t '==>' t'" (at level 40).
+Inductive bigstep : exp -> exp -> Prop :=
+  | ST_Val : forall n t1 t2 w1 w2,
+    <{t1}> ==> <{w1}> ->
+    <{/n := w1/ t2 }> ==> <{w2}> ->
+    <{val n = t1 ; t2}> ==> <{w2}>
+  | ST_App : forall v t1 t2' t2 w,
+    value v ->
+    <{t1}> ==> v ->
+    <{t2}> ==> <{t2'}> ->
+    <{v t2'}> ==> <{w}> ->
+    <{t1 t2}> ==> <{w}>
+  | ST_Fun : forall n x T2 t1 v w,
+    value v ->
+    <{ /n:=(fun n [x:T2] {t1})/ /x:=v/ t1 }> ==> <{w}> ->
+    <{(fun n [x:T2] {t1}) v}> ==> <{w}>
+  | ST_Succ: forall (n:nat) w e, 
+    w = S n ->
+    <{e}> ==> <{n}> ->
+    <{succ e}> ==> <{w}>
+  | ST_Pred: forall (n:nat) w e, 
+    w = Nat.pred n ->
+    <{e}> ==> <{n}> ->
+    <{pred e}> ==> <{w}>
+  | ST_Prod: forall n (n':nat) m (m':nat) w, 
+    w = n' * m' ->
+    <{n}> ==> <{n'}> ->
+    <{m}> ==> <{m'}> ->
+    <{n * m}> ==> <{w}>
+  | ST_If_T: forall t1 t2 t3,
+    <{t1}> ==> <{true}> ->
+    <{if t1 then t2 else t3}> ==> <{t2}>
+  | ST_If_F: forall t1 t2 t3,
+    <{t1}> ==> <{false}> ->
+    <{if t1 then t2 else t3}> ==> <{t3}>
+  | ST_Refl: forall t1, <{t1}> ==> <{t1}>
+where "t '==>' t'" := (bigstep t t').
