big_step_semantics_test.v
@@ -1,0 +1,53 @@
+Require Import expression.
+Require Import big_step_semantics.
+Require Import String.
+
+(*NOTATION*)
+Definition x : string := "x".
+Definition y : string := "y".
+Definition z : string := "z".
+Definition n : string := "n".
+Definition fun0: string := "fun0". 
+Definition prod5: string := "prod5". 
+
+Hint Unfold x : core.
+Hint Unfold y : core.
+Hint Unfold z : core.
+
+(*Test of pred succ*)
+Lemma bigstep_pred_succ:forall (i:nat), <{pred (succ i)}> ==> <{i}>.
+Proof.
+intro i.
+apply ST_Pred with (n:=(S i)).
+-simpl. reflexivity.
+-apply ST_Succ with (n:=i). reflexivity. apply ST_Refl.
+Qed.
+
+(*Test of val*)
+Lemma bigstep_val: <{val n = (5*5) ; n * 2}> ==> 50.
+Proof.
+apply ST_Val with (w1:=25). 
+-apply ST_Prod with (n':=5)( m':=5). reflexivity. apply ST_Refl. apply ST_Refl.
+-simpl. apply ST_Prod with (n':=25)( m':=2). simpl. reflexivity. apply ST_Refl. apply ST_Refl.
+Qed.
+
+(*Test of fun*)
+Lemma bigstep_fun: <{fun prod5 [x:Nat] {x * 5} 5}> ==> 25.
+Proof.
+apply ST_Fun. simpl.
+- apply v_nat.
+- simpl. apply ST_Prod with (n':=5)(m':=5). reflexivity. apply ST_Refl. apply ST_Refl.
+Qed.
+
+Notation "'const' x " := (l_succ x) (in custom acnotation at level 0,
+                                     x custom acnotation at level 0).
+
+(*Test of fun*)
+Lemma bigstep_nv_fun: <{fun prod5 [x:Nat] {x * [> 5 ]} ([>5])}> ==> <{[>5]*[>5]}>.
+Proof.
+apply ST_Fun. simpl.
+- apply v_nvalue.
+- simpl. apply ST_Refl.
+Qed.
+
+
