value_tree.v
@@ -1,15 +1,13 @@
 Require Import String. 
 Require Import nvalue. 
 Require Import PeanoNat. 
+Require Import List. 
 
 Inductive value_tree: Type :=
-| empty : list0 -> value_tree
-| some (B:Type) (A:nvalue B): list0  -> value_tree
-with list0 :=
-| nill : list0
-| cons : value_tree -> list0 -> list0.
+| empty : list value_tree -> value_tree
+| some (B:Type) (A:nvalue B): list value_tree  -> value_tree.
 
-Definition extract_l (v:value_tree) : list0:= 
+Definition extract_l (v:value_tree) : list value_tree:= 
 match v with 
 | empty l => l
 | some _ _ l => l
